src/LifetimePerms.v
@@ -1317,5 +1317,8 @@ Section LifetimePerms.
     red in H.
 
   Qed.
-*)
+ *)
+
+
+
 End LifetimePerms.
