src2/SepStep2.v
@@ -1,0 +1,939 @@
+(* begin hide *)
+From Coq Require Import
+     Classes.Morphisms
+     Classes.RelationClasses
+     Relations.Relation_Operators
+     Relations.Operators_Properties.
+(* end hide *)
+
+Section step.
+  Context {config : Type}.
+
+  (** * Rely-guarantee permissions *)
+  Record perm : Type :=
+    {
+      inv : config -> Prop;
+      (** The rely: the updates this permission allows of others. *)
+      rely : config -> config -> Prop;
+      rely_PO : PreOrder rely;
+      (** The guarantee: the updates that this permission allows. *)
+      guar : config -> config -> Prop;
+      guar_PO : PreOrder guar;
+      (** The precondition on configs. *)
+      pre : config -> Prop;
+      pre_respects : forall x y, rely x y -> pre x -> pre y;
+
+      inv_rely : forall x y, rely x y -> inv x -> inv y;
+      inv_guar : forall x y, guar x y -> inv x -> inv y;
+    }.
+  Global Instance rely_is_preorder p : PreOrder (rely p) := rely_PO p.
+  Global Instance guar_is_preorder p : PreOrder (guar p) := guar_PO p.
+
+  (** ** Separate permissions *)
+  Record separate (p q : perm) : Prop :=
+    {
+      sep_l: forall x y, inv q x -> inv p x ->
+                    guar q x y -> rely p x y;
+      sep_r: forall x y, inv p x -> inv q x ->
+                    guar p x y -> rely q x y;
+    }.
+
+  Notation "p ⊥ q" := (separate p q) (at level 50).
+
+  Global Instance separate_symmetric: Symmetric separate.
+  Proof.
+    intros p q []. constructor; auto.
+  Qed.
+
+  (** * Preserves separability *)
+  Definition sep_step (p q : perm) : Prop :=
+    forall r, p ⊥ r -> q ⊥ r.
+
+  Global Instance sep_step_refl : Reflexive sep_step.
+  Proof.
+    repeat intro; auto.
+  Qed.
+
+  Global Instance sep_step_trans : Transitive sep_step.
+  Proof.
+    repeat intro. auto.
+  Qed.
+
+  Program Definition bottom_perm : perm :=
+    {|
+      pre x := True;
+      rely x y := True;
+      guar := eq;
+      inv x := True;
+    |}.
+  Next Obligation.
+    constructor; repeat intro; subst; auto.
+  Qed.
+
+  Lemma bottom_perm_is_bottom : forall p, sep_step p bottom_perm.
+  Proof.
+    split; intros; cbn in *; subst; auto. reflexivity.
+  Qed.
+
+  Lemma separate_bottom : forall p, p ⊥ bottom_perm.
+  Proof.
+    constructor; intros; simpl; auto. cbn in *. subst.
+    reflexivity.
+  Qed.
+
+  Program Definition top_perm : perm :=
+    {|
+      pre x := False;
+      rely x y := x = y;
+      guar x y := True;
+      inv x := True;
+    |}.
+  Next Obligation.
+    constructor; repeat intro; subst; auto.
+  Qed.
+
+  Lemma top_perm_is_top : forall p, sep_step top_perm p.
+  Proof.
+    split; intros; cbn in *.
+    - apply H in H2; cbn; auto. cbn in H2. subst. reflexivity.
+    - apply H; cbn; auto.
+  Qed.
+
+  Program Definition sym_guar_perm (p : perm) : perm :=
+    {|
+      pre x := False;
+      rely := guar p;
+      guar := rely p;
+      inv x := inv p x;
+    |}.
+  Next Obligation.
+    eapply inv_guar; eauto.
+  Qed.
+  Next Obligation.
+    eapply inv_rely; eauto.
+  Qed.
+  Lemma separate_sym_guar : forall p, p ⊥ sym_guar_perm p.
+  Proof.
+    intros. split; intros; auto.
+  Qed.
+
+  Program Definition sym_guar_perm' (p : perm) : perm :=
+    {|
+      pre x := False;
+      rely := guar p;
+      guar := rely p;
+      inv x := True;
+    |}.
+  Lemma separate_sym_guar' : forall p, p ⊥ sym_guar_perm' p.
+  Proof.
+    intros. split; intros; auto.
+  Qed.
+  (* Program Definition sym_guar_perm' (p : perm) : perm := *)
+  (*   {| *)
+  (*     pre x := False; *)
+  (*     rely x y := guar p x y /\ inv p x; *)
+  (*     guar x y := x = y \/ rely p x y /\ inv p x; *)
+  (*     inv x := inv p x; *)
+  (*   |}. *)
+  (* Next Obligation. *)
+  (*   constructor; repeat intro. *)
+  (*   left. reflexivity. destruct H, H0; subst; auto. destruct H, H0. *)
+  (*   right. split; auto. etransitivity; eauto. *)
+  (* Qed. *)
+  (* Next Obligation. *)
+  (*   constructor; repeat intro. *)
+  (*   left. reflexivity. destruct H, H0; subst; auto. destruct H, H0. *)
+  (*   right. split; auto. etransitivity; eauto. *)
+  (* Qed. *)
+  (* Next Obligation. *)
+  (*   destruct H; subst; auto. destruct H. eapply inv_guar; eauto. *)
+  (* Qed. *)
+  (* Next Obligation. *)
+  (*   destruct H; subst; auto. destruct H. eapply inv_rely; eauto. *)
+  (* Qed. *)
+  (* Lemma separate_sym_guar' : forall p, p ⊥ sym_guar_perm' p. *)
+  (* Proof. *)
+  (*   intros. split; cbn; intros; auto. *)
+  (*   destruct H1; subst. reflexivity. *)
+  (*   destruct H1; auto. *)
+  (* Qed. *)
+
+
+  (* guar gets smaller *)
+  Lemma sep_step_guar : forall p q x y, sep_step p q ->
+                                  (* inv p x -> *)
+                                  inv q x ->
+                                  guar q x y ->
+                                  guar p x y.
+  Proof.
+    intros. specialize (H (sym_guar_perm' p) (separate_sym_guar' p)).
+    apply H; cbn; auto.
+  Qed.
+
+  (* rely gets bigger *)
+  Lemma sep_step_rely : forall p q x y, sep_step p q ->
+                                   inv q x ->
+                                   (* inv p x -> *)
+                                   rely p x y ->
+                                   rely q x y.
+  Proof.
+    intros. specialize (H (sym_guar_perm' p) (separate_sym_guar' _)).
+    apply H; cbn; auto.
+  Qed.
+(*
+  Program Definition sym_guar_inv_perm (p : perm) : perm :=
+    {|
+      pre x := False;
+      rely x y := inv p x <-> inv p y;
+      guar x y := inv p x <-> inv p y;
+      inv x := True;
+    |}.
+  Next Obligation.
+    constructor; repeat intro; split; auto.
+    - intros. apply H0. apply H; auto.
+    - intros. apply H. apply H0; auto.
+  Qed.
+  Next Obligation.
+    constructor; repeat intro; split; auto.
+    - intros. apply H0. apply H; auto.
+    - intros. apply H. apply H0; auto.
+  Qed.
+
+  Lemma sep_step_inv_guar : forall p q x, sep_step p q ->
+                                       inv q x ->
+                                       (* guar q x y -> *)
+                                       inv p x.
+  Proof.
+    intros. specialize (H (sym_guar_inv_perm p)).
+    destruct H. admit.
+    cbn in *.
+    destruct H. cbn in *.
+    specialize (sep_r0 x x).
+    destruct sep_r0; auto.
+  Qed.
+
+  Lemma sep_step_rg : forall p q,
+      (forall x y, guar q x y -> guar p x y) ->
+      (forall x y, rely p x y -> rely q x y) ->
+      sep_step p q.
+  Proof.
+    repeat intro. split; intros.
+    - apply H0. apply H1; auto.
+    - apply H1. apply H. auto.
+  Qed.
+
+  Lemma sep_step_iff : forall p q,
+      sep_step p q <-> (forall x y, rely p x y -> rely q x y) /\ (forall x y, guar q x y -> guar p x y).
+  Proof.
+    split; [split; intros; [eapply sep_step_rely | eapply sep_step_guar] |
+            intros []; apply sep_step_rg]; eauto.
+  Qed.
+
+  Lemma sep_step_sep_conj_l : forall p1 p2 q, p1 ⊥ q -> sep_step p1 p2 -> sep_step (p1 ** q) (p2 ** q).
+  Proof.
+    intros p1 p2 q ? ?.
+    repeat intro; auto. symmetry in H1. symmetry. apply separate_sep_conj_perm; symmetry; auto.
+    - apply H0. symmetry. eapply separate_sep_conj_perm_l; eauto.
+    - symmetry. eapply separate_sep_conj_perm_r; eauto.
+  Qed.
+  Lemma sep_step_sep_conj_r : forall p1 p2 q, p1 ⊥ q -> sep_step p1 p2 -> sep_step (q ** p1) (q ** p2).
+  Proof.
+    intros p1 p2 q ? ?.
+    repeat intro; auto. symmetry in H1. symmetry. apply separate_sep_conj_perm; symmetry; auto.
+    - symmetry. eapply separate_sep_conj_perm_l; eauto.
+    - apply H0. symmetry. eapply separate_sep_conj_perm_r; eauto.
+    - symmetry. auto.
+  Qed.
+ *)
+
+  Lemma separate_antimonotone : forall p q r, p ⊥ q -> sep_step q r -> p ⊥ r.
+  Proof.
+    intros. symmetry. apply H0. symmetry; auto.
+  Qed.
+
+  (** ** Separating conjunction for permissions *)
+  Program Definition sep_conj_perm (p q: perm) : perm :=
+    {|
+      pre := fun x => pre p x /\ pre q x;
+      rely := fun x y => rely p x y /\ rely q x y;
+      guar := clos_trans _ (fun x y => (guar p x y) \/ (guar q x y)) (* separateness implies each move is in the others' rely *) ;
+      inv := fun x => inv p x /\ inv q x /\ p ⊥ q;
+    |}.
+  Next Obligation.
+    constructor; repeat intro.
+    - split; reflexivity.
+    - destruct H, H0.
+      split; etransitivity; eauto.
+  Qed.
+  Next Obligation.
+    constructor.
+    - constructor; intuition.
+    - repeat intro. destruct H, H0.
+      + destruct H, H0; econstructor 2; constructor; eauto.
+      + econstructor 2. left. apply H. econstructor 2; eauto.
+      + econstructor 2; eauto. econstructor 2; eauto. left. assumption.
+      + repeat (econstructor 2; eauto).
+  Qed.
+  Next Obligation.
+    split; eapply pre_respects; eauto.
+  Qed.
+  Next Obligation.
+    split; [| split]; auto; eapply inv_rely; eauto.
+  Qed.
+  Lemma inv_clos_trans p q x y :
+    inv p x ->
+    inv q x ->
+    p ⊥ q ->
+    clos_trans config (fun x y : config => guar p x y \/ guar q x y) x y ->
+    inv p y /\ inv q y.
+  Proof.
+    intros Hp Hq Hsep H. induction H; intros.
+    - destruct H.
+      + split; [eapply inv_guar; eauto |].
+        apply Hsep in H; auto. eapply inv_rely; eauto.
+      + split; [| eapply inv_guar; eauto].
+        apply Hsep in H; auto. eapply inv_rely; eauto.
+    - apply IHclos_trans2; apply IHclos_trans1; auto.
+  Qed.
+  Next Obligation.
+    destruct (inv_clos_trans _ _ _ _ H0 H1 H2 H); auto.
+  Qed.
+  Notation "p ** q" := (sep_conj_perm p q) (at level 40).
+
+  Lemma sep_conj_perm_commut p q :
+    sep_step (p ** q) (q ** p).
+  Proof.
+    split; repeat intro.
+    - destruct H1 as (? & ? & ?). apply H in H2; auto.
+      2: { split; [| split]; auto. symmetry. auto. }
+      destruct H2. split; auto.
+    - destruct H0 as (? & ? & ?).
+      apply H; auto.
+      { split; [| split]; auto. symmetry. auto. }
+      clear H0 H3 H4 H1.
+      induction H2; auto.
+      + destruct H0; constructor; [right | left]; auto.
+      + etransitivity; eauto.
+  Qed.
+
+  Lemma clos_trans_guar_eq p x y :
+    clos_trans config (fun x y : config => x = y \/ guar p x y) x y ->
+    guar p x y.
+  Proof.
+    intros. induction H.
+    - destruct H; auto. subst. reflexivity.
+    - etransitivity; eauto.
+  Qed.
+
+  Lemma sep_conj_perm_bottom : forall p, sep_step (p ** bottom_perm) p.
+  Proof.
+    split; intros; cbn in *; subst; auto.
+    - apply H in H2; auto. destruct H2; auto.
+      split; [| split]; cbn; auto. apply separate_bottom.
+    - apply H; auto. split; [| split]; cbn; auto. apply separate_bottom.
+      constructor. left. auto.
+  Qed.
+  Lemma sep_conj_perm_bottom' : forall p, sep_step p (p ** bottom_perm).
+  Proof.
+    split; intros; cbn in *; subst; auto.
+    - split; auto. apply H; auto. apply H1.
+    - apply H; auto. apply H0.
+      clear H H0 H1. induction H2.
+      destruct H; auto. subst. reflexivity.
+      etransitivity; eauto.
+  Qed.
+  (* Lemma sep_conj_perm_top : forall p, sep_step (p ** top_perm) top_perm. *)
+  (* Proof. *)
+  (*   split; intros; cbn in *; subst; auto. *)
+  (*   - apply H in H2; auto. destruct H2; auto. *)
+  (*     split; [| split]; auto. 2: { *)
+  (*   - apply H; auto. split; [| split]; cbn; auto. apply separate_bottom. *)
+  (*     constructor. left. auto. *)
+  (* Qed. *)
+
+  Program Definition inv_perm (inv : config -> Prop) : perm :=
+    {|
+      pre x := False;
+      rely x y := inv x -> inv y;
+      guar x y := x = y;
+      inv := inv;
+    |}.
+  Next Obligation.
+    constructor; repeat intro; auto.
+  Qed.
+  (* Next Obligation. *)
+  (*   constructor; repeat intro; auto. *)
+  (* Qed. *)
+
+  (* sep_step q (inv q) + "frame rule" would imply this *)
+  Lemma sep_step_sep_conj_l p q (Hsep : p ⊥ q) :
+    sep_step (p ** q) (inv_perm (inv q) ** p).
+  Proof.
+    repeat intro.
+    (* destruct H. *)
+    split; intros.
+    - cbn in *. destruct H1 as (? & ? & ?). apply H in H2; auto.
+      2: { cbn. auto. }
+      destruct H2.
+      split; auto. intros. eapply inv_rely; eauto.
+    - destruct H0 as (? & ? & ?). cbn in *. apply H; auto.
+      split; [| split]; auto.
+      constructor 1. left.
+      apply clos_trans_guar_eq; auto.
+  Qed.
+
+  Lemma sep_step_inv_perm p i :
+    sep_step (p ** inv_perm i) p.
+  Proof.
+    split; repeat intro.
+    - apply H; auto. cbn. admit.
+    - apply H; auto. admit.
+  Abort.
+
+  (** * Permission sets *)
+  (** Perms = upwards-closed sets of permissions *)
+  Record Perms :=
+    {
+      in_Perms : perm -> Prop;
+      Perms_upwards_closed : forall p1 p2, in_Perms p1 -> sep_step p2 p1 -> in_Perms p2
+    }.
+  Notation "p ∈ P" := (in_Perms P p) (at level 60).
+  (** ** Permission set ordering *)
+  (** Defined as superset. *)
+  Definition lte_Perms (P Q : Perms) : Prop :=
+    forall p, p ∈ Q -> p ∈ P.
+  Notation "P ⊑ Q" := (lte_Perms P Q) (at level 60).
+
+  Global Instance lte_Perms_is_preorder : PreOrder lte_Perms.
+  Proof.
+    constructor; repeat intro; auto.
+  Qed.
+
+  (** Various lattice definitions. *)
+  Program Definition top_Perms : Perms :=
+    {|
+    in_Perms := fun r => False
+    |}.
+
+  Lemma top_Perms_is_top : forall P, P ⊑ top_Perms.
+  Proof.
+    repeat intro. inversion H.
+  Qed.
+
+  Program Definition bottom_Perms : Perms :=
+    {|
+    in_Perms := fun r => True
+    |}.
+
+  Lemma bottom_Perms_is_bottom : forall P, bottom_Perms ⊑ P.
+  Proof.
+    repeat intro. simpl. auto.
+  Qed.
+
+  (** The least Perms set containing a given p *)
+  Program Definition singleton_Perms p1 : Perms :=
+    {|
+    in_Perms := fun p2 => sep_step p2 p1
+    |}.
+  Next Obligation.
+    etransitivity; eassumption.
+  Qed.
+
+  Program Definition join_Perms (Ps : Perms -> Prop) : Perms :=
+    {|
+    in_Perms := fun p => forall P, Ps P -> p ∈ P
+    |}.
+  Next Obligation.
+    eapply Perms_upwards_closed; eauto.
+  Qed.
+  Lemma lte_join_Perms : forall (Ps : Perms -> Prop) P,
+      Ps P ->
+      P ⊑ join_Perms Ps.
+  Proof.
+    repeat intro. apply H0. auto.
+  Qed.
+  Lemma join_Perms_min : forall (Ps : Perms -> Prop) Q,
+      (forall P, Ps P -> P ⊑ Q) ->
+      join_Perms Ps ⊑ Q.
+  Proof.
+    repeat intro.
+    eapply H; eauto.
+  Qed.
+
+  (** Complete meet of Perms sets = union *)
+  Program Definition meet_Perms (Ps : Perms -> Prop) : Perms :=
+    {|
+    in_Perms := fun p => exists P, Ps P /\ p ∈ P
+    |}.
+  Next Obligation.
+    exists H. split; auto.
+    apply (Perms_upwards_closed _ p1); assumption.
+  Qed.
+
+  Lemma lte_meet_Perms : forall (Ps : Perms -> Prop) P,
+      Ps P ->
+      meet_Perms Ps ⊑ P.
+  Proof.
+    repeat intro. exists P. auto.
+  Qed.
+
+  Lemma meet_Perms_max : forall (Ps : Perms -> Prop) Q,
+      (forall P, Ps P -> Q ⊑ P) ->
+      Q ⊑ meet_Perms Ps.
+  Proof.
+    repeat intro. destruct H0 as [? [? ?]].
+    eapply H; eauto.
+  Qed.
+
+  Definition meet_Perms2 P Q : Perms := meet_Perms (fun R => R = P \/ R = Q).
+
+  (** Set equality *)
+  Definition eq_Perms (P Q : Perms) : Prop := P ⊑ Q /\ Q ⊑ P.
+  Notation "P ≡ Q" := (eq_Perms P Q) (at level 60).
+
+  Global Instance Equivalence_eq_Perms : Equivalence eq_Perms.
+  Proof.
+    constructor; repeat intro.
+    - split; reflexivity.
+    - destruct H; split; auto.
+    - destruct H, H0. split; etransitivity; eauto.
+  Qed.
+
+  Global Instance Proper_eq_Perms_lte_Perms :
+    Proper (eq_Perms ==> eq_Perms ==> Basics.flip Basics.impl) lte_Perms.
+  Proof.
+    do 5 red. intros. etransitivity. apply H. etransitivity. apply H1. apply H0.
+  Qed.
+
+  Global Instance Proper_eq_Perms_eq_perm_in_Perms : Proper (eq_Perms ==> eq ==> Basics.flip Basics.impl) in_Perms.
+  Proof.
+    repeat intro; subst. apply H. auto.
+  Qed.
+
+  (** ** Separating conjunction for permission sets *)
+  Program Definition sep_conj_Perms (P Q : Perms) : Perms :=
+    {|
+    in_Perms := fun r => exists p q, p ∈ P /\ q ∈ Q /\ p ⊥ q /\ sep_step r (p ** q)
+    |}.
+  Next Obligation.
+    exists H, H1. split; [| split; [| split]]; auto. etransitivity; eauto.
+  Qed.
+  Notation "P * Q" := (sep_conj_Perms P Q).
+
+  (* Lemma lte_l_sep_conj_Perms : forall P Q, P ⊑ P * Q. *)
+  (* Proof. *)
+  (*   intros P Q p' ?. destruct H as (p & q & Hp & Hq & ? & ?). *)
+  (*   eapply Perms_upwards_closed; eauto. *)
+  (*   etransitivity; eauto. apply lte_l_sep_conj_perm. *)
+  (* Qed. *)
+
+  (* Lemma lte_r_sep_conj_Perms : forall P Q, Q ⊑ P * Q. *)
+  (* Proof. *)
+  (*   intros P Q p' ?. destruct H as (p & q & Hp & Hq & ? & ?). *)
+  (*   eapply Perms_upwards_closed; eauto. *)
+  (*   etransitivity; eauto. apply lte_r_sep_conj_perm. *)
+  (* Qed. *)
+
+  (* Lemma sep_conj_Perms_bottom_identity : forall P, bottom_Perms * P ≡ P. *)
+  (* Proof. *)
+  (*   constructor; repeat intro. *)
+  (*   - exists bottom_perm, p. split; cbn; [| split; [| split]]; auto. *)
+  (*     + symmetry. apply separate_bottom. *)
+  (*     + etransitivity. 2: apply sep_conj_perm_commut. apply sep_conj_perm_bottom'. *)
+  (*   - destruct H as (? & ? & ? & ? & ? & ?).  *)
+  (*     eapply (Perms_upwards_closed P); eauto. *)
+  (*     etransitivity; eauto. apply lte_r_sep_conj_perm. *)
+  (* Qed. *)
+
+  Lemma sep_conj_Perms_top_absorb : forall P, top_Perms * P ≡ top_Perms.
+  Proof.
+    constructor; repeat intro.
+    - inversion H.
+    - destruct H as [? [_ [[] _]]].
+  Qed.
+
+  Lemma sep_conj_Perms_monotone : forall P P' Q Q', P' ⊑ P -> Q' ⊑ Q -> P' * Q' ⊑ P * Q.
+  Proof.
+    repeat intro. destruct H1 as [? [? [? [? ?]]]].
+    exists x, x0. auto.
+  Qed.
+
+  Lemma sep_conj_Perms_perm: forall P Q p q,
+      p ∈ P ->
+      q ∈ Q ->
+      p ⊥ q ->
+      p ** q ∈ P * Q.
+  Proof.
+    intros. exists p, q. split; [| split; [| split]]; auto. reflexivity.
+  Qed.
+
+
+End step.
+
+Notation "p ⊥ q" := (separate p q) (at level 50).
+Notation "p ** q" := (sep_conj_perm p q) (at level 40).
+Notation "p ∈ P" := (in_Perms P p) (at level 60).
+Notation "P ⊑ Q" := (lte_Perms P Q) (at level 60).
+Notation "P ≡ Q" := (eq_Perms P Q) (at level 60).
+Notation "P * Q" := (sep_conj_Perms P Q).
+
+Notation "P ⊨ Q" := (lte_Perms Q P) (at level 60).
+
+From Heapster Require Import
+  Utils.
+
+From ITree Require Import
+     ITree
+     ITreeFacts
+     Basics.MonadState
+     Basics.MonadProp
+     Events.State
+     Events.Exception
+     Events.Nondeterminism
+     Eq.Eqit
+     Eq.UpToTaus
+     Eq.EqAxiom.
+
+From Paco Require Import
+     paco.
+
+Import ITreeNotations.
+Local Open Scope itree_scope.
+
+Ltac rewritebisim lem := pose proof lem as bisim;
+                         eapply bisimulation_is_eq in bisim;
+                         rewrite bisim;
+                         clear bisim.
+
+Ltac rewritebisim_in lem H := pose proof lem as bisim;
+                              eapply bisimulation_is_eq in bisim;
+                              rewrite bisim in H;
+                              clear bisim.
+
+Lemma throw_vis {E R} `{exceptE unit -< E} (k : void -> itree E R) :
+  vis (Throw tt) k = throw tt.
+Proof.
+  apply bisimulation_is_eq. pstep. unfold throw.
+  constructor. intros. inversion v.
+Qed.
+
+Lemma throw_bind {E R1 R2} `{exceptE unit -< E} (k : R1 -> itree E R2) :
+  x <- throw tt;; k x = throw tt.
+Proof.
+  unfold throw. rewritebisim @bind_vis. apply throw_vis.
+Qed.
+
+(** * Stuttering bisimulation *)
+Section bisim.
+  Context {config specConfig : Type}.
+
+  Inductive sbuter_gen {R1 R2 : Type} (sbuter : perm -> (R1 -> R2 -> Perms) -> itree (sceE config) R1 -> config -> itree (sceE specConfig) R2 -> specConfig -> Prop)
+            (p : perm) (Q : R1 -> R2 -> Perms) :
+    itree (sceE config) R1 -> config -> itree (sceE specConfig) R2 -> specConfig -> Prop :=
+  | sbuter_gen_ret r1 c1 r2 c2 :
+      pre p (c1, c2) ->
+      p ∈ Q r1 r2 ->
+      sbuter_gen sbuter p Q (Ret r1) c1 (Ret r2) c2
+  | sbuter_gen_err t1 c1 c2 :
+      sbuter_gen sbuter p Q t1 c1 (throw tt) c2
+  | sbuter_gen_tau_L t1 c1 t2 c2 :
+      pre p (c1, c2) ->
+      sbuter_gen sbuter p Q t1 c1 t2 c2 ->
+      sbuter_gen sbuter p Q (Tau t1) c1 t2 c2
+  | sbuter_gen_tau_R t1 c1 t2 c2 :
+      pre p (c1, c2) ->
+      sbuter_gen sbuter p Q t1 c1 t2 c2 ->
+      sbuter_gen sbuter p Q t1 c1 (Tau t2) c2
+  | sbuter_gen_tau t1 c1 t2 c2 :
+      pre p (c1, c2) ->
+      sbuter p Q t1 c1 t2 c2 ->
+      sbuter_gen sbuter p Q (Tau t1) c1 (Tau t2) c2
+  | sbuter_gen_modify_L f k c1 t2 c2 p' :
+      pre p (c1, c2) ->
+      guar p (c1, c2) (f c1, c2) ->
+      sep_step p p' ->
+      sbuter_gen sbuter p' Q (k c1) (f c1) t2 c2 ->
+      sbuter_gen sbuter p Q (vis (Modify f) k) c1 t2 c2
+  | sbuter_gen_modify_R t1 c1 f k c2 p' :
+      pre p (c1, c2) ->
+      guar p (c1, c2) (c1, f c2) ->
+      sep_step p p' ->
+      sbuter_gen sbuter p' Q t1 c1 (k c2) (f c2) ->
+      sbuter_gen sbuter p Q t1 c1 (vis (Modify f) k) c2
+  | sbuter_gen_modify f1 k1 c1 f2 k2 c2 p' :
+      pre p (c1, c2) ->
+      guar p (c1, c2) (f1 c1, f2 c2) ->
+      sep_step p p' ->
+      (* TODO: f1 c1 satisfies the spred *)
+      sbuter p' Q (k1 c1) (f1 c1) (k2 c2) (f2 c2) ->
+      sbuter_gen sbuter p Q (vis (Modify f1) k1) c1 (vis (Modify f2) k2) c2
+  | sbuter_gen_choice_L k c1 t2 c2 p' :
+      pre p (c1, c2) ->
+      sep_step p p' ->
+      (forall b, sbuter_gen sbuter p' Q (k b) c1 t2 c2) ->
+      sbuter_gen sbuter p Q (vis Or k) c1 t2 c2
+  | sbuter_gen_choice_R t1 c1 k c2 p' :
+      pre p (c1, c2) ->
+      sep_step p p' ->
+      (forall b, sbuter_gen sbuter p' Q t1 c1 (k b) c2) ->
+      sbuter_gen sbuter p Q t1 c1 (vis Or k) c2
+  | sbuter_gen_choice k1 c1 k2 c2 p' :
+      pre p (c1, c2) ->
+      sep_step p p' ->
+      (forall b1, exists b2, sbuter p' Q (k1 b1) c1 (k2 b2) c2) ->
+      (forall b2, exists b1, sbuter p' Q (k1 b1) c1 (k2 b2) c2) ->
+      sbuter_gen sbuter p Q (vis Or k1) c1 (vis Or k2) c2
+  .
+
+  Lemma sbuter_gen_mon {R1 R2} : monotone6 (@sbuter_gen R1 R2).
+  Proof.
+    repeat intro. induction IN; subst; try solve [econstructor; eauto]; auto.
+    econstructor 11; eauto; intros.
+    - destruct (H1 b1). eexists; eauto.
+    - destruct (H2 b2). eexists; eauto.
+  Qed.
+  #[local] Hint Resolve sbuter_gen_mon : paco.
+
+  Definition sbuter {R1 R2} := paco6 (@sbuter_gen R1 R2) bot6.
+
+  Lemma sbuter_gen_pre {R1 R2} r p (Q : R1 -> R2 -> Perms) t s c1 c2 :
+    sbuter_gen r p Q t c1 s c2 ->
+    s = throw tt \/ pre p (c1, c2).
+  Proof.
+    inversion 1; auto.
+  Qed.
+
+  Lemma sbuter_lte {R1 R2} p Q Q' (t : itree (sceE config) R1) (s : itree (sceE specConfig) R2) c1 c2 :
+    sbuter p Q t c1 s c2 -> (forall r1 r2, Q r1 r2 ⊨ Q' r1 r2) -> sbuter p Q' t c1 s c2.
+  Proof.
+    revert p Q Q' t s c1 c2. pcofix CIH. intros p Q Q' t s c1 c2 Htyping Hlte.
+    punfold Htyping. pstep.
+    induction Htyping; pclearbot; try solve [econstructor; eauto].
+    - constructor; eauto. apply Hlte. auto.
+    - econstructor 11; eauto; intros.
+      + destruct (H1 b1). eexists. right. eapply CIH; eauto. pclearbot. apply H3.
+      + destruct (H2 b2). eexists. right. eapply CIH; eauto. pclearbot. apply H3.
+  Qed.
+
+  (** * Typing *)
+  Definition typing {R1 R2} P Q (t : itree (sceE config) R1) (s : itree (sceE specConfig) R2) :=
+    forall p c1 c2, p ∈ P -> pre p (c1, c2) -> sbuter p Q t c1 s c2.
+  (* TODO: add inv here *)
+
+  Lemma typing_lte {R1 R2} P P' Q Q' (t : itree (sceE config) R1) (s : itree (sceE specConfig) R2) :
+    typing P Q t s ->
+    P' ⊨ P ->
+    (forall r1 r2, Q r1 r2 ⊨ Q' r1 r2) ->
+    typing P' Q' t s.
+  Proof.
+    repeat intro.
+    eapply sbuter_lte; eauto.
+  Qed.
+
+  Lemma typing_ret {R1 R2} P Q (r1 : R1) (r2 : R2) :
+    P ⊨ Q r1 r2 -> typing P Q (Ret r1) (Ret r2).
+  Proof.
+    repeat intro. pstep. constructor; auto.
+  Qed.
+
+  Lemma rewrite_spin {E R} : (ITree.spin : itree E R) = Tau (ITree.spin).
+  Proof.
+    intros. apply bisimulation_is_eq.
+    ginit. gcofix CIH. gstep. unfold ITree.spin. constructor.
+    apply Reflexive_eqit_gen_eq.
+  Qed.
+  Lemma typing_spin {R1 R2} P Q :
+    typing P Q (ITree.spin : itree (sceE config) R1) (ITree.spin : itree (sceE specConfig) R2).
+  Proof.
+    repeat intro. pcofix CIH. pstep.
+    rewrite (@rewrite_spin _ R1). rewrite (@rewrite_spin _ R2).
+    constructor 5; auto.
+  Qed.
+
+  Lemma typing_top {R1 R2} Q (t : itree (sceE config) R1) (s : itree (sceE specConfig) R2) :
+    typing top_Perms Q t s.
+  Proof.
+    repeat intro. inversion H.
+  Qed.
+
+  Lemma sbuter_bottom {R1 R2} p Q (t : itree (sceE config) R1) (s : itree (sceE specConfig) R2) c1 c2:
+    sbuter p Q t c1 s c2 -> sbuter p (fun _ _ => bottom_Perms) t c1 s c2.
+  Proof.
+    revert p Q t s c1 c2. pcofix CIH. intros. pstep. punfold H0.
+    induction H0; pclearbot; try solve [econstructor; simpl; eauto].
+    econstructor 11; eauto; intros.
+    - destruct (H1 b1). eexists. right. eapply CIH; pclearbot; apply H3.
+    - destruct (H2 b2). eexists. right. eapply CIH; pclearbot; apply H3.
+  Qed.
+
+  Lemma typing_bottom {R1 R2} P Q (t : itree (sceE config) R1) (s : itree (sceE specConfig) R2) :
+    typing P Q t s -> typing P (fun _ _ => bottom_Perms) t s.
+  Proof.
+    repeat intro. eapply sbuter_bottom; eauto.
+  Qed.
+
+  Lemma sbuter_bind {R1 R2 S1 S2} (p : perm) (Q : R1 -> S1 -> Perms) (R : R2 -> S2 -> Perms)
+        (t1 : itree (sceE config) R1) (t2 : R1 -> itree (sceE config) R2)
+        (s1 : itree (sceE specConfig) S1) (s2 : S1 -> itree (sceE specConfig) S2)
+        c1 c2 r :
+    pre p (c1, c2) ->
+    sbuter p Q t1 c1 s1 c2 ->
+    (forall r1 r2 p c1 c2, p ∈ (Q r1 r2) ->
+                      pre p (c1, c2) ->
+                      paco6 sbuter_gen r p R (t2 r1) c1 (s2 r2) c2) ->
+    paco6 sbuter_gen r p R (x <- t1 ;; t2 x) c1 (x <- s1 ;; s2 x) c2.
+  Proof.
+    revert p Q R t1 t2 s1 s2 c1 c2. pcofix CIH.
+    intros p Q R t1 t2 s1 s2 c1 c2 Hpre Htyping1 Htyping2.
+    punfold Htyping1. induction Htyping1.
+    - do 2 rewritebisim @bind_ret_l. specialize (Htyping2 _ _ _ c1 c2 H0 H).
+      eapply paco6_mon; eauto.
+    - rewrite throw_bind. pstep. constructor.
+    - rewritebisim @bind_tau.
+      specialize (IHHtyping1 Hpre Htyping2). punfold IHHtyping1.
+      pstep. constructor; auto.
+    - rewritebisim @bind_tau.
+      specialize (IHHtyping1 Hpre Htyping2). punfold IHHtyping1.
+      pstep. constructor; auto.
+    - do 2 rewritebisim @bind_tau. pclearbot.
+      pstep. constructor 5; auto. right. eapply CIH; eauto.
+    - rewritebisim @bind_vis. apply sbuter_gen_pre in Htyping1. destruct Htyping1; subst.
+      + rewrite throw_bind. pstep. constructor.
+      + specialize (IHHtyping1 H2 Htyping2). punfold IHHtyping1. pstep. econstructor; eauto.
+    - rewritebisim @bind_vis. apply sbuter_gen_pre in Htyping1. destruct Htyping1; subst.
+      + pstep. econstructor; eauto. rewrite H2. rewrite throw_bind. constructor.
+      + specialize (IHHtyping1 H2 Htyping2). punfold IHHtyping1. pstep. econstructor; eauto.
+    - do 2 rewritebisim @bind_vis. pclearbot.
+      pose proof H2. punfold H2.
+      pstep. econstructor 8; eauto.
+      destruct (sbuter_gen_pre _ _ _ _ _ _ _ H2); eauto.
+      rewrite H4. rewrite throw_bind. left. pstep. constructor.
+    - rewritebisim @bind_vis. pstep. econstructor; eauto. intros.
+      destruct (sbuter_gen_pre _ _ _ _ _ _ _ (H1 b)).
+      + rewrite H3. rewrite throw_bind. constructor.
+      + specialize (H2 b H3 Htyping2). punfold H2.
+    - rewritebisim @bind_vis. pstep. econstructor; eauto. intros.
+      destruct (sbuter_gen_pre _ _ _ _ _ _ _ (H1 b)).
+      + rewrite H3. rewrite throw_bind. constructor.
+      + specialize (H2 b H3 Htyping2). punfold H2.
+    - do 2 rewritebisim @bind_vis. pclearbot. pstep. econstructor 11; eauto; intros.
+      + specialize (H1 b1). destruct H1. pclearbot.
+        punfold H1. destruct (sbuter_gen_pre _ _ _ _ _ _ _ H1).
+        * exists x. left. pstep. rewrite H3. rewrite throw_bind. econstructor; eauto.
+        * eexists. right. eapply CIH; eauto. pstep; eauto.
+      + specialize (H2 b2). destruct H2. pclearbot.
+        punfold H2. destruct (sbuter_gen_pre _ _ _ _ _ _ _ H2).
+        * exists x. left. pstep. rewrite H3. rewrite throw_bind. econstructor; eauto.
+        * eexists. right. eapply CIH; eauto. pstep; eauto.
+  Qed.
+
+  Lemma typing_bind {R1 R2 S1 S2} (P : Perms) (Q : R1 -> S1 -> Perms) (R : R2 -> S2 -> Perms)
+        (t1 : itree (sceE config) R1) (t2 : R1 -> itree (sceE config) R2)
+        (s1 : itree (sceE specConfig) S1) (s2 : S1 -> itree (sceE specConfig) S2) :
+    typing P Q t1 s1 ->
+    (forall r1 r2, typing (Q r1 r2) R (t2 r1) (s2 r2)) ->
+    typing P R (x <- t1 ;; t2 x) (x <- s1 ;; s2 x).
+  Proof.
+    repeat intro.
+    eapply sbuter_bind; eauto.
+  Qed.
+
+  Lemma sbuter_frame {R1 R2} p r p' Q R (t : itree (sceE config) R1) (s : itree (sceE specConfig) R2) c1 c2:
+    pre p' (c1, c2) ->
+    inv p' (c1, c2) ->
+    r ∈ R ->
+    sep_step p' (p ** r) ->
+    sbuter p Q t c1 s c2 ->
+    sbuter p' (fun r1 r2 => Q r1 r2 * R) t c1 s c2.
+  Proof.
+    revert p r p' Q R t s c1 c2. pcofix CIH. rename r into r0.
+    intros p r p' Q R t s c1 c2 Hpre Hinv Hr Hlte Hsbuter. pstep. punfold Hsbuter.
+    revert p' Hlte Hpre Hinv. generalize dependent r.
+    induction Hsbuter; intros; pclearbot; try solve [econstructor; eauto].
+    - constructor; auto. eapply Perms_upwards_closed; eauto.
+      apply sep_conj_Perms_perm; auto.
+
+      (* do 2 eexists. split; [| split; [| split]]; eauto. *)
+      (* apply Hlte in Hpre. apply Hpre. *)
+      (* reflexivity. *)
+    - apply sbuter_gen_pre in Hsbuter. destruct Hsbuter; [subst; constructor |].
+      econstructor; eauto.
+      + apply Hlte. constructor. left. auto.
+      + eapply sep_step_lte; eauto. apply sep_step_sep_conj_l; eauto.
+        apply Hlte in Hpre. apply Hpre.
+      + eapply IHHsbuter; eauto. reflexivity.
+        split; [| split]; auto.
+        * apply Hlte in Hpre. destruct Hpre as (? & ? & ?). respects.
+          apply H5. auto.
+        * apply H1. apply Hlte in Hpre. apply Hpre.
+    - econstructor; eauto.
+      + apply Hlte. constructor. left. auto.
+      + eapply sep_step_lte; eauto. apply sep_step_sep_conj_l; eauto.
+        apply Hlte in Hpre. apply Hpre.
+      + apply sbuter_gen_pre in Hsbuter. destruct Hsbuter; [rewrite H2; constructor |].
+        eapply IHHsbuter; eauto. reflexivity.
+        split; [| split]; auto.
+        * apply Hlte in Hpre. destruct Hpre as (? & ? & ?). respects.
+          apply H5. auto.
+        * apply H1. apply Hlte in Hpre. apply Hpre.
+    - econstructor 8; eauto.
+      3: { pose proof H2 as Hsbuter.
+           punfold Hsbuter. apply sbuter_gen_pre in Hsbuter.
+           destruct Hsbuter; [rewrite H3; left; pstep; constructor |].
+           right. eapply CIH. 4: apply H2. 2: eauto. 2: reflexivity.
+           apply Hlte in Hpre. destruct Hpre as (? & ? & ?).
+           split; [| split]; auto.
+           respects. apply H6. auto.
+      }
+      + apply Hlte. constructor. left. auto.
+      + eapply sep_step_lte; eauto. apply sep_step_sep_conj_l; auto.
+        apply Hlte in Hpre. apply Hpre.
+    - econstructor; eauto.
+      + eapply sep_step_lte; eauto. apply sep_step_sep_conj_l; eauto.
+        apply Hlte in Hpre. apply Hpre.
+      + intros. specialize (H1 b).
+        apply sbuter_gen_pre in H1. destruct H1; [subst; constructor |].
+        eapply H2; eauto. reflexivity.
+        apply Hlte in Hpre. destruct Hpre as (? & ? & ?).
+        split; [| split]; auto.
+    - econstructor; eauto.
+      + eapply sep_step_lte; eauto. apply sep_step_sep_conj_l; eauto.
+        apply Hlte in Hpre. apply Hpre.
+      + intros. specialize (H1 b).
+        apply sbuter_gen_pre in H1. destruct H1; [rewrite H1; constructor |].
+        eapply H2; eauto. reflexivity.
+        apply Hlte in Hpre. destruct Hpre as (? & ? & ?).
+        split; [| split]; auto.
+    - econstructor 11; eauto.
+      2: { intros. specialize (H1 b1). destruct H1 as (b2 & H1). pclearbot. exists b2.
+           pose proof H1 as Hsbuter.
+           punfold Hsbuter. apply sbuter_gen_pre in Hsbuter.
+           destruct Hsbuter; [rewrite H3; left; pstep; constructor |].
+           right. eapply CIH. 4: apply H1. 2: eauto. 2: reflexivity.
+           apply Hlte in Hpre. destruct Hpre as (? & ? & ?).
+           split; [| split]; auto.
+      }
+      2: { intros. specialize (H2 b2). destruct H2 as (b1 & H2). pclearbot. exists b1.
+           pose proof H2 as Hsbuter.
+           punfold Hsbuter. apply sbuter_gen_pre in Hsbuter.
+           destruct Hsbuter; [rewrite H3; left; pstep; constructor |].
+           right. eapply CIH. 4: apply H2. 2: eauto. 2: reflexivity.
+           apply Hlte in Hpre. destruct Hpre as (? & ? & ?).
+           split; [| split]; auto.
+      }
+      eapply sep_step_lte; eauto. apply sep_step_sep_conj_l; auto.
+      apply Hlte in Hpre. apply Hpre.
+  Qed.
+
+  Lemma typing_frame {R1 R2} P Q R (t : itree (sceE config) R1) (s : itree (sceE specConfig) R2):
+    typing P Q t s ->
+    typing (P * R) (fun r1 r2 => Q r1 r2 * R) t s.
+  Proof.
+    intros Ht p' c1 c2 (p & r & Hp & Hr & Hsep & Hlte) Hpre.
+    pose proof Hpre as H. apply Hlte in H. destruct H as (Hprep & Hprer & Hsep').
+    eapply sbuter_frame; eauto.
+  Qed.
+
+
+
+End bisim.
